$E\times B $drift velocity

$\vec{v} =  -c\{B_z+\frac{mc}{q}(\frac{cE_A\sin\{2\pi(\frac{t}{T}-\frac{R_0\theta}{\lambda})+\frac{\pi}{2}\}}{B_z^2} \xi_r)\}^{-1}(E_A\sin\{2\pi(\frac{t}{T}-\frac{R_0\theta}{\lambda})+\frac{\pi}{2}\}-\frac{\mu}{q}\xi_r+\frac{mc^2}{q}\frac{(E_A\sin\{2\pi(\frac{t}{T}-\frac{R_0\theta}{\lambda})+\frac{\pi}{2}\})^2\xi_r}{B_z^3})\vec{e_\theta}$

if electric field is constant,


$\vec{v} =  -c\{B_z+\frac{mc}{q}(\frac{cE_A}{B_z^2} \xi_r)\}^{-1}(E_A-\frac{\mu}{q}\xi_r+\frac{mc^2}{q}\frac{(E_A)^2\xi_r}{B_z^3})\vec{e_\theta}$

assumption: E_A $3\mathrm{mV/m}$


$3\mathrm{mV} = 3\times10^{-3}\times\frac{10^8}{3.0\times10^{10}}\mathrm{statV} = 10^{-5}\mathrm{statV}$

$3\mathrm{mV/m} = 10^{-7}\mathrm{statV/cm}$


assumption $B_z = \frac{B_E}{L^3}$ (in magnetic equator) , $B_E = 3.11\times10^{-5}\mathrm{T}= 3.11\times10^{-1}\mathrm{G}$
if $L = 6$, $B_z = 1.4\times10^{-7}\mathrm{T} = 1.4\times10^{-3}\mathrm{G}$

assumption : $v_\perp = 0.01c = 3.0\times10^8\mathrm{cm/s}$

$\mu = \frac{mv_{\perp}^2}{2B_z} = \frac{(9.1\times 10^{-28}\mathrm{g})\times(3.0\times10^8\mathrm{cm/s})^2}{2.0\times1.4\times10^{-3}\mathrm{G}}$

$\xi_r = \frac{\partial B_z}{\partial r} = \frac{\partial B_z}{\partial L}\frac{\partial L}{\partial r} =-3\frac{B_E}{L^4}\frac{1}{R_0} = \frac{-3\times 3.1\times 10^{-1}\mathrm{G}}{6^4\times6\times10^8\mathrm{cm}}$



$\{B_z+\frac{mc}{q}(\frac{cE_A}{B_z^2} \xi_r)\} = 1.4\times10^{-3}\mathrm{G} + \frac{9.1\times 10^{-28}\mathrm{g}\times3.0\times10^{10}\mathrm{cm/s}}{4.8\times10^{-10}\mathrm{statC}}(\frac{3.0\times10^{10}\mathrm{cm/s}\times10^{-7}\mathrm{statV/cm}}{(1.4\times10^{-3}\mathrm{G})^2}\frac{-3\times 3.1\times 10^{-1}\mathrm{G}}{6^4\times6\times10^8\mathrm{cm}}) = 1.4\times10^{-3}\mathrm{G}-\frac{9.1\times3.0\times3.0\times3\times3.1}{4.8\times1.4\times1.4\times6^4\times6}\frac{10^{-16}}{10^{-8}}=1.4\times10^{-3}\mathrm{G}-0.01\times10^{-8}\mathrm{G}$

about $(E_A-\frac{\mu}{q}\xi_r+\frac{mc^2}{q}\frac{(E_A)^2\xi_r}{B_z^3})\vec{e_\theta}$

$E_A = 10^{-7}\mathrm{statV/cm}$

$\frac{\mu}{q}\xi_r =\frac{(9.1\times 10^{-28}\mathrm{g})\times(3.0\times10^8\mathrm{cm/s})^2}{2.0\times1.4\times10^{-3}\mathrm{G}}\times\frac{1}{4.8\times10^{-10}\mathrm{statC}} \times \frac{-3\times 3.1\times 10^{-1}\mathrm{G}}{6^4\times6\times10^8\mathrm{cm}} = -\frac{9.1\times3.0\times3.0\times3\times3.1}{2.0\times1.4\times4.8\times6^4\times6}\times\frac{10^{-13}}{10^{-5}}\mathrm{statV/cm} = -0.0073\times10^{-8}\mathrm{statV/cm} = -7.3\times10^{-11}\mathrm{statV/cm}$

$\frac{mc^2}{q}\frac{(E_A)^2\xi_r}{B_z^3} = \frac{mc}{q}(\frac{c(E_A)^2\xi_r}{B_z^3}) =  \{ \frac{mc}{q}(\frac{cE_A\xi_r}{B_z^2}) \}(\frac{E_A}{B_z}) = -(0.01\times10^{-8}\mathrm{G})\times\frac{10^{-7}\mathrm{statV/cm}}{1.4\times 10^{-3}\mathrm{G}} =- \frac{1}{1.4}\times 10^{-14}\mathrm{statV/cm} = -7.1\times10^{-15}\mathrm{statV/cm}$


$v =  -c\{B_z+\frac{mc}{q}(\frac{cE_A}{B_z^2} \xi_r)\}^{-1}(E_A-\frac{\mu}{q}\xi_r+\frac{mc^2}{q}\frac{(E_A)^2\xi_r}{B_z^3}) = c\frac{( 10^{-7}\mathrm{statV/cm}-7.3\times10^{-11}\mathrm{statV/cm}-7.1\times10^{-15}\mathrm{statV/cm})}{1.4\times10^{-3}\mathrm{G}-0.01\times10^{-6}\mathrm{G}} = 3.0\times10^{10}\mathrm{cm/s}\times(7.1\times10^{-5}-5.2\times10^{-8}-5.0\times10^{-12}) =(2.1\times10^{6}-1.6\times10^{3}-1.5\times10^{-1})\mathrm{cm/s}$

from Basic space plasma physics

$|\vec{v_E}| = v_E = \frac{E}{B} = \frac{3\mathrm{mV/m}}{1.4\times10^{-7}T} = 2.1\times10^4\mathrm{m/s}$