# Parameter standardization

Definition

$c$ : lightspeed

$m = m_e m^\ast$

$q = q_e q^\ast$

$v = cv^\ast$

$T$ ULF wave period

$x = c Tx^\ast$

$\vec{B} = B_{eq}\vec{B^\ast}$

$\vec{E} = B_{eq}\vec{E^\ast}$

$t = Tt^\ast$   


$\frac{\partial B_z}{\partial r} = \xi_r$


so,

$\frac{\partial (B_z^\ast B_{eq})}{\partial (cTr^\ast)} = \frac{ B_{eq}}{cT}\frac{\partial B_z^\ast}{\partial r^\ast}  =  \frac{ B_{eq}}{cT}\xi_r^\ast = \xi_r$


$\vec{v} =  -\{B_z+\frac{mc}{q}(\frac{cE_A\sin\{2\pi(\frac{t}{T}-\frac{R_0\theta}{\lambda})+\frac{\pi}{2}\}}{B_z^2} \xi_r)\}^{-1}(E_A\sin\{2\pi(\frac{t}{T}-\frac{R_0\theta}{\lambda})+\frac{\pi}{2}\}-\frac{\mu}{q}\xi_r+\frac{mc^2}{q}\frac{(E_A\sin\{2\pi(\frac{t}{T}-\frac{R_0\theta}{\lambda})+\frac{\pi}{2}\})^2\xi_r}{B_z^3})\vec{e_\theta}$



$\vec{v} =  -\{B_{eq}B_z^\ast+\frac{m_e m^\ast c}{q_e q^\ast}(\frac{cB_{eq}E_A^\ast\sin\{2\pi(\frac{Tt^\ast}{T}-\frac{R_0\theta}{\lambda})+\frac{\pi}{2}\}}{(B_z^\ast B_{eq})^2} \frac{ B_{eq}}{cT}\xi_r^\ast )\}^{-1}(B_{eq}E_A^\ast\sin\{2\pi(\frac{Tt^\ast}{T}-\frac{R_0\theta}{\lambda})+\frac{\pi}{2}\}-\frac{\mu}{ q_e q^\ast} \frac{ B_{eq}}{cT}\xi_r^\ast+\frac{ m_e m^\ast c^2}{ q_e q^\ast}\frac{(B_{eq}E_A^\ast\sin\{2\pi(\frac{Tt^\ast}{T}-\frac{R_0\theta}{\lambda})+\frac{\pi}{2}\})^2\frac{ B_{eq}}{cT}\xi_r^\ast }{(B_z^\ast B_{eq})^3})\vec{e_\theta}$


$\vec{v} =  -\{B_{eq}B_z^\ast+\frac{m_e m^\ast c}{q_e q^\ast}(\frac{E_A^\ast\sin\{2\pi(t^\ast-\frac{R_0\theta}{\lambda})+\frac{\pi}{2}\}}{(B_z^\ast )^2} \frac{1}{T}\xi_r^\ast )\}^{-1}(B_{eq}E_A^\ast\sin\{2\pi(t^\ast-\frac{R_0\theta}{\lambda})+\frac{\pi}{2}\}-\frac{\mu}{ q_e q^\ast} \frac{ B_{eq}}{cT}\xi_r^\ast+\frac{ m_e m^\ast c^2 }{ q_e q^\ast}\frac{(E_A^\ast\sin\{2\pi(t^\ast-\frac{R_0\theta}{\lambda})+\frac{\pi}{2}\})^2\frac{1}{T}\xi_r^\ast }{(B_z^\ast)^3})\vec{e_\theta}$


$\vec{v} =  -\{B_z^\ast+\frac{m_e m^\ast c}{B_{eq}q_e q^\ast}(\frac{E_A^\ast\sin\{2\pi(t^\ast-\frac{R_0\theta}{\lambda})+\frac{\pi}{2}\}}{(B_z^\ast )^2} \frac{1}{T}\xi_r^\ast )\}^{-1}(E_A^\ast\sin\{2\pi(t^\ast-\frac{R_0\theta}{\lambda})+\frac{\pi}{2}\}-\frac{\mu}{ q_e q^\ast} \frac{1}{cT}\xi_r^\ast+\frac{ m_e m^\ast c^2}{ q_e q^\ast B_{eq}}\frac{(E_A^\ast\sin\{2\pi(t^\ast-\frac{R_0\theta}{\lambda})+\frac{\pi}{2}\})^2\frac{1}{T}\xi_r^\ast }{(B_z^\ast)^3})\vec{e_\theta}$

$\Omega_e = \frac{q_e}{cm_e}B_{eq}$ : Electron cyclotron frequency

$\vec{v} =  -\{B_z^\ast+\frac{m^\ast}{\Omega_e q^\ast}(\frac{E_A^\ast\sin\{2\pi(t^\ast-\frac{R_0\theta}{\lambda})+\frac{\pi}{2}\}}{(B_z^\ast )^2} \frac{1}{T}\xi_r^\ast )\}^{-1}(E_A^\ast\sin\{2\pi(t^\ast-\frac{R_0\theta}{\lambda})+\frac{\pi}{2}\}-\frac{\mu}{ q_e q^\ast} \frac{1}{cT}\xi_r^\ast+\frac{m^\ast c}{\Omega_e q^\ast}\frac{(E_A^\ast\sin\{2\pi(t^\ast-\frac{R_0\theta}{\lambda})+\frac{\pi}{2}\})^2\frac{1}{T}\xi_r^\ast }{(B_z^\ast)^3})\vec{e_\theta}$

$\mu = \frac{mv_\perp^2}{2B} = \frac{m^\ast m_e c^2 v^{\ast 2}_\perp }{2B^\ast B_{eq}} =\frac{c^2m_e}{B_{eq}}\frac{m^\ast v^{\ast 2}_\perp}{2B^\ast} =\frac{c^2m_e}{B_{eq}}\mu^\ast$


$\vec{v} =  -\{B_z^\ast+\frac{m^\ast}{\Omega_e q^\ast}(\frac{E_A^\ast }{(B_z^\ast )^2}\sin\{2\pi(t^\ast-\frac{R_0\theta}{\lambda})+\frac{\pi}{2}\} \frac{1}{T}\xi_r^\ast )\}^{-1}(E_A^\ast\sin\{2\pi(t^\ast-\frac{R_0\theta}{\lambda})+\frac{\pi}{2}\}-\frac{m_e c^2 }{B_{eq}}\mu^\ast\frac{1}{ q_e q^\ast} \frac{1}{cT}\xi_r^\ast+\frac{m^\ast c}{\Omega_e q^\ast}\frac{1}{(B_z^\ast)^3}(E^\ast_A\sin\{2\pi(t^\ast-\frac{R_0\theta}{\lambda})+\frac{\pi}{2}\})^2\frac{1}{T}\xi_r^\ast )\vec{e_\theta}$

$\vec{v} =  -\{B_z^\ast+\frac{m^\ast}{\Omega_e q^\ast}(\frac{E_A^\ast }{(B_z^\ast )^2}\sin\{2\pi(t^\ast-\frac{R_0\theta}{\lambda})+\frac{\pi}{2}\} \frac{1}{T}\xi_r^\ast )\}^{-1}(E_A^\ast\sin\{2\pi(t^\ast-\frac{R_0\theta}{\lambda})+\frac{\pi}{2}\}-\frac{\mu^\ast}{  q^\ast \Omega_e}\frac{1}{T}\xi_r^\ast+\frac{m^\ast c}{\Omega_e q^\ast}\frac{1}{(B_z^\ast)^3}(E^\ast_A\sin\{2\pi(t^\ast-\frac{R_0\theta}{\lambda})+\frac{\pi}{2}\})^2\frac{1}{T}\xi_r^\ast )\vec{e_\theta}$

$\vec{v} =  -\{B_z^\ast+\frac{m^\ast}{q^\ast}\frac{\xi_r^\ast }{T \Omega_e }(\frac{E_A^\ast }{(B_z^\ast )^2}\sin\{2\pi(t^\ast-\frac{R_0\theta}{\lambda})+\frac{\pi}{2}\})\}^{-1}(E_A^\ast\sin\{2\pi(t^\ast-\frac{R_0\theta}{\lambda})+\frac{\pi}{2}\}-\frac{\mu^\ast}{  q^\ast}\frac{\xi_r^\ast}{T \Omega_e}+\frac{m^\ast c}{q^\ast}\frac{1}{(B_z^\ast)^3}\frac{\xi_r^\ast}{T \Omega_e}(E^\ast_A\sin\{2\pi(t^\ast-\frac{R_0\theta}{\lambda})+\frac{\pi}{2}\})^2 )\vec{e_\theta}$

$\vec{v^\ast} =  -\frac{1}{c}\{B_z^\ast+\frac{m^\ast}{q^\ast}\frac{\xi_r^\ast }{T \Omega_e }(\frac{E_A^\ast }{(B_z^\ast )^2}\sin\{2\pi(t^\ast-\frac{R_0\theta}{\lambda})+\frac{\pi}{2}\})\}^{-1}(E_A^\ast\sin\{2\pi(t^\ast-\frac{R_0\theta}{\lambda})+\frac{\pi}{2}\}-\frac{\mu^\ast}{  q^\ast}\frac{\xi_r^\ast}{T \Omega_e}+\frac{m^\ast c}{q^\ast}\frac{1}{(B_z^\ast)^3}\frac{\xi_r^\ast}{T \Omega_e}(E^\ast_A\sin\{2\pi(t^\ast-\frac{R_0\theta}{\lambda})+\frac{\pi}{2}\})^2 )\vec{e_\theta}$