# Guiding Center Equation

reference :: https://agupubs.onlinelibrary.wiley.com/doi/full/10.1029/2010JA015682

$\frac{\partial f}{\partial t}+\vec{v} \cdot \frac{\partial f}{\partial \vec{x}}+\dot{v_\parallel}\frac{\partial f}{\partial v_\parallel} = 0$

$\vec{v} = v_\parallel\frac{\vec{B}^\ast}{B^\ast_\parallel}+\frac{\vec{D}}{B_\parallel^\ast}\times\vec{b}$

$\dot{v}_ \parallel = \frac{q}{m}\vec{D}\cdot\frac{\vec{B}^\ast}{{B^\ast}_\parallel}$


$\vec{D} = \vec{E}-\frac{\mu}{q}\nabla \vec{B} - \frac{m}{q}(v_\parallel\frac{\partial b}{\partial t}+\frac{\partial \vec{v_E}}{\partial t}+\nabla \frac{v_E^2}{2})$

$\vec{v_E} =\frac{\vec{E}}{B} \times \vec{b}$

$\vec{B^\ast} = \vec{B} + \frac{m}{q}(v_\parallel \nabla \times \vec{b}+\nabla\times\vec{v_E})$

$B^\ast_\parallel = \vec{B^\ast} \cdot \vec{b}$

$B = |\vec{B}|$


if pitch angle is 90 degree, $v_\parallel = 0$

$\frac{\partial f}{\partial t}+\vec{v} \cdot \frac{\partial f}{\partial \vec{x}}= 0$

$\vec{v} = \frac{\vec{D}}{B_\parallel^\ast}\times\vec{b}$

$\vec{D} =\vec{E}-\frac{\mu}{q}\nabla \vec{B} - \frac{m}{q}(\frac{\partial \vec{v_E}}{\partial t}+\nabla \frac{v_E^2}{2})$

$\vec{v_E} =\frac{\vec{E}}{B} \times \vec{b}$

$\vec{B^\ast} = \vec{B} + \frac{m}{q}(\nabla\times\vec{v_E})$

$B^\ast_\parallel = \vec{B^\ast} \cdot \vec{b}$

$B = |\vec{B}|$


